verify apowSubtract, building my way to lemmas for apow for all integers

math/Artin2_1.dfy
@@ -1,164 +1,275 @@
+module Artin {
+    //!A signifies type invariance
+    datatype Group<!A> = Group(elements: set<A>, identity: A, compose: (A,A) -> A, inverse: (A) -> A)
 
-//!A signifies type invariance
-datatype Group<!A> = Group(elements: set<A>, identity: A, compose: (A,A) -> A, inverse: (A) -> A)
-
-predicate isIdentity<A>(g: Group<A>) {
-    forall a :: a in g.elements ==> g.compose(a,g.identity) == a && g.compose(g.identity, a) == a
-}
-
-predicate closedComposition<A>(g: Group<A>) {
-    forall x,y :: x in g.elements && y in g.elements ==> g.compose(x,y) in g.elements
-}
-
-predicate associativeComposition<A>(g: Group<A>) {
-    forall a,b,c :: a in g.elements && b in g.elements && c in g.elements ==> g.compose(g.compose(a,b),c) == g.compose(a, g.compose(b,c))
-}
-
-predicate commutativeComposition<A>(g: Group<A>) {
-    forall a,b :: a in g.elements && b in g.elements ==> g.compose(a,b) == g.compose(b,a)
-}
-
-//problematic, aka recursive trigger, it generates new patterns that match the trigger
-predicate containsInverses<A>(g: Group<A>) {
-    forall x :: x in g.elements ==> exists xbar :: xbar in g.elements && g.compose(x,xbar) == g.identity
-}
-predicate PleaseInstantiateMe<A>(x: A) {
-    true
-}
-
-//no longer blocks apowAddition, but doesn't help groupCompositionInverse
-// predicate containsInverses<A>(g: Group<A>) {
-//   forall x {:trigger PleaseInstantiateMe(x)} :: 
-//     PleaseInstantiateMe(x) && x in g.elements ==> 
-//     exists xbar :: 
-//       xbar in g.elements && g.compose(x,xbar) == g.identity
-// }
-predicate closedInverse<A>(g: Group<A>) {
-  forall x {:trigger g.inverse(x)} :: x in g.elements ==> g.inverse(x) in g.elements
-}
-
-predicate isInverse<A>(g: Group<A>) {
-  forall x {:trigger g.inverse(x)} :: x in g.elements ==> g.compose(x,g.inverse(x)) == g.identity && g.compose(g.inverse(x),x) == g.identity
-}
-
-predicate ValidGroup<A>(g: Group<A>) {
-    g.identity in g.elements &&
-    isIdentity(g) &&
-    closedComposition(g) &&
-    associativeComposition(g) &&
-    closedInverse(g) &&
-    isInverse(g)
-    // containsInverses(g)
-}
-
-predicate ValidSubGroup<A>(g: Group<A>, h: Group<A>) {
-    h.elements <= g.elements &&
-    g.identity in h.elements &&
-    g.identity == h.identity &&
-    g.compose == h.compose &&
-    closedComposition(h) //&&
-    // containsInverses(h)
-}
-
-predicate AbelianGroup<A>(g: Group<A>) {
-    ValidGroup(g) && commutativeComposition(g)
-}
-
-lemma {:verify true} groupCompositionInverse<A>(g: Group<A>, a: A, b: A, abar: A, bbar: A, abbar: A)
-    requires ValidGroup(g)
-    requires a in g.elements
-    requires b in g.elements
-    requires g.inverse(a) == abar
-    requires g.inverse(b) == bbar
-    requires g.inverse(g.compose(a,b)) == abbar
-    ensures abbar == g.compose(bbar, abar)
-{
-    calc {
-        g.compose(g.compose(a, b), g.compose(bbar, abar));
-        ==
-        g.compose(a, g.compose(g.compose(b, bbar),abar));
-        ==
-        g.compose(a, g.compose(g.identity,abar));
-        ==
-        g.compose(a, abar);
-        ==
-        g.identity;
+    predicate isIdentity<A>(g: Group<A>) {
+        forall a :: a in g.elements ==> g.compose(a,g.identity) == a && g.compose(g.identity, a) == a
     }
-}
 
-//apow is short for abstract power
-function apow<A>(g: Group, elem: A, n: nat): A
-    requires elem in g.elements
-{
-    if n == 0 then g.identity else g.compose(elem, apow(g, elem, n-1))
-}
-
-lemma onePower<A>(g: Group, elem: A)
-    requires elem in g.elements
-    requires isIdentity(g)
-    ensures apow(g, elem, 1) == elem;
-{
-    calc {
-        apow(g, elem, 1);
-        g.compose(elem, apow(g, elem, 0));
-        g.compose(elem, g.identity);
-        elem;
+    predicate closedComposition<A>(g: Group<A>) {
+        forall x,y :: x in g.elements && y in g.elements ==> g.compose(x,y) in g.elements
     }
-}
 
-lemma apowClosed<A>(g: Group, elem: A, n: nat)
-    requires elem in g.elements
-    requires g.identity in g.elements
-    requires isIdentity(g)
-    requires closedComposition(g)
-    ensures apow(g, elem, n) in g.elements
-{}
+    predicate associativeComposition<A>(g: Group<A>) {
+        forall a,b,c :: a in g.elements && b in g.elements && c in g.elements ==> g.compose(g.compose(a,b),c) == g.compose(a, g.compose(b,c))
+    }
 
-lemma {:verify true} apowAddition<A>(g: Group<A>, elem: A, n: nat, k: nat)
-    requires elem in g.elements
-    requires ValidGroup(g)
-    ensures g.compose(apow(g, elem, n), apow(g, elem, k)) == apow(g, elem, n+k)
-{
-    apowClosed(g, elem, n);
-    apowClosed(g, elem, k);
-    if k == 0 {
-        assert apow(g, elem, k) == g.identity;
-        assert g.compose(apow(g, elem, n), g.identity) == apow(g, elem, n+k);
-    }else if n == 0 {
-        assert apow(g, elem, n) == g.identity;
-        assert g.compose(g.identity, apow(g, elem, k)) == apow(g, elem, n+k);
-    }else{
-        apowClosed(g, elem, n-1);
-        apowClosed(g, elem, n+k);
+    predicate commutativeComposition<A>(g: Group<A>) {
+        forall a,b :: a in g.elements && b in g.elements ==> g.compose(a,b) == g.compose(b,a)
+    }
+
+    //problematic, aka recursive trigger, it generates new patterns that match the trigger
+    predicate containsInverses<A>(g: Group<A>) {
+        forall x :: x in g.elements ==> exists xbar :: xbar in g.elements && g.compose(x,xbar) == g.identity
+    }
+    predicate PleaseInstantiateMe<A>(x: A) {
+        true
+    }
+
+    //no longer blocks apowAddition, but doesn't help groupCompositionInverse
+    // predicate containsInverses<A>(g: Group<A>) {
+    //   forall x {:trigger PleaseInstantiateMe(x)} :: 
+    //     PleaseInstantiateMe(x) && x in g.elements ==> 
+    //     exists xbar :: 
+    //       xbar in g.elements && g.compose(x,xbar) == g.identity
+    // }
+    predicate closedInverse<A>(g: Group<A>) {
+    forall x {:trigger g.inverse(x)} :: x in g.elements ==> g.inverse(x) in g.elements
+    }
+
+    predicate isInverse<A>(g: Group<A>) {
+    forall x {:trigger g.inverse(x)} :: x in g.elements ==> g.compose(x,g.inverse(x)) == g.identity && g.compose(g.inverse(x),x) == g.identity
+    }
+
+    predicate ValidGroup<A>(g: Group<A>) {
+        g.identity in g.elements &&
+        isIdentity(g) &&
+        closedComposition(g) &&
+        associativeComposition(g) &&
+        closedInverse(g) &&
+        isInverse(g)
+        // containsInverses(g)
+    }
+
+    predicate ValidSubGroup<A>(g: Group<A>, h: Group<A>) {
+        h.elements <= g.elements &&
+        g.identity in h.elements &&
+        g.identity == h.identity &&
+        g.compose == h.compose &&
+        closedComposition(h) //&&
+        // containsInverses(h)
+    }
+
+    predicate AbelianGroup<A>(g: Group<A>) {
+        ValidGroup(g) && commutativeComposition(g)
+    }
+
+    lemma {:verify true} groupCompositionInverse<A>(g: Group<A>, a: A, b: A, abar: A, bbar: A, abbar: A)
+        requires ValidGroup(g)
+        requires a in g.elements
+        requires b in g.elements
+        requires g.inverse(a) == abar
+        requires g.inverse(b) == bbar
+        requires g.inverse(g.compose(a,b)) == abbar
+        ensures abbar == g.compose(bbar, abar)
+    {
         calc {
-            g.compose(apow(g, elem, n), apow(g, elem, k));
-            g.compose(g.compose(elem, apow(g, elem, n-1)), apow(g, elem, k));
-            g.compose(elem, g.compose(apow(g, elem, n-1), apow(g, elem, k)));
-            == {apowAddition(g,elem, n-1,k);}
-            g.compose(elem, apow(g, elem, n-1+k));
-            apow(g, elem, n+k);
+            g.compose(g.compose(a, b), g.compose(bbar, abar));
+            ==
+            g.compose(a, g.compose(g.compose(b, bbar),abar));
+            ==
+            g.compose(a, g.compose(g.identity,abar));
+            ==
+            g.compose(a, abar);
+            ==
+            g.identity;
         }
     }
+
+    //apow is short for abstract power
+    function apow<A>(g: Group, elem: A, n: int): A
+        requires elem in g.elements
+        decreases n*n
+        ensures n == 0 ==> apow(g,elem,n) == g.identity
+    {
+        if n == 0 then g.identity else if n > 0 then g.compose(elem, apow(g, elem, n-1)) else if n < 0 then g.compose(g.inverse(elem), apow(g, elem, n+1)) else g.identity
+    }
+
+    lemma apowPos<A>(g: Group, elem: A, n: int)
+        requires elem in g.elements
+        requires n > 0
+        ensures n > 0 ==> apow(g,elem,n) == g.compose(elem, apow(g, elem, n-1))
+    {}
+
+    lemma apowNegative<A>(g: Group, elem: A, n: int)
+        requires elem in g.elements
+        requires !(n > 0)
+        ensures n < 0 ==> apow(g,elem,n) == g.compose(g.inverse(elem), apow(g, elem, n+1))
+    {}
+
+
+    lemma onePower<A>(g: Group, elem: A)
+        requires elem in g.elements
+        requires isIdentity(g)
+        ensures apow(g, elem, 1) == elem;
+    {
+        calc {
+            apow(g, elem, 1);
+            g.compose(elem, apow(g, elem, 0));
+            g.compose(elem, g.identity);
+            elem;
+        }
+    }
+
+    lemma oneMinusPower<A>(g: Group, elem: A)
+        requires elem in g.elements
+        requires isIdentity(g)
+        requires closedInverse(g) && isInverse(g)
+        ensures apow(g, elem, -1) == g.inverse(elem);
+    {
+    }
+
+    lemma {:verify true} apowClosed<A>(g: Group, elem: A, n: int)
+        requires elem in g.elements
+        requires g.identity in g.elements
+        requires isIdentity(g)
+        requires closedComposition(g)
+        requires closedInverse(g)
+        requires isInverse(g)
+        // requires n >= 0
+        decreases n*n
+        ensures apow(g, elem, n) in g.elements
+    {
+        // if n == 0 {
+        //     assert apow(g, elem, 0) in g.elements;
+        // } else if n > 0 {
+        //     // apowPos(g, elem, n);
+        //     // apowClosed(g, elem, n-1);
+        // }else {
+        //     apowNegative(g,elem, n);
+        //     apowClosed(g, elem, n+1);
+        //     assert apow(g, elem, n+1) in g.elements;
+        //     assert elem in g.elements;
+        //     // calc {
+        //     //     apow(g, elem, n);
+        //     //     g.compose(g.inverse(elem), )
+        //     // }
+        //     assert apow(g, elem, n) in g.elements;
+        // }
 }
 
-predicate CyclicGroupGeneratedBy<A(!new)>(g: Group, elem: A)
-    requires elem in g.elements
-{
-    exists n :: n == |g.elements| &&
-        apow(g, elem, n) == g.identity &&
-        (forall ns :: ns != n && apow(g, elem, ns) == g.identity ==> n < ns) &&
-        n != 0 &&
-        forall x :: x in g.elements && exists n :: apow(g, elem, n) == x
-}
+    lemma {:verify true} allApowClosed<A>(g: Group, elem: A) 
+        requires ValidGroup(g)
+        requires elem in g.elements
+        ensures forall x: int :: apow(g, elem, x) in g.elements
+    {
+        forall x: int | true 
+        {
+            apowClosed(g, elem, x);
+        }
+    }
 
-lemma {:verify false} AllSubgroupsOfCyclicSubgroupsAreCyclic<A(!new)>(g: Group, elem: A, h:Group)
-    requires elem in g.elements
-    requires CyclicGroupGeneratedBy(g, elem)
-    requires ValidGroup(g)
-    requires h.elements <= g.elements
-    requires ValidGroup(h)
-    requires ValidSubGroup(g, h)
-    ensures exists hx: A :: hx in h.elements && CyclicGroupGeneratedBy(h, hx)
-{
+    // method {:verify true} apowSubtract<A>(g: Group<A>, elem: A, n: int)
+    lemma {:verify true} {:induction false} apowSubtract<A>(g: Group<A>, elem: A, n: int)
+        requires ValidGroup(g)
+        requires elem in g.elements
+        requires n >= 0
+        // ensures g.compose(apow(g, elem, n), apow(g, elem, -1)) == apow(g, elem, n-1)
+        ensures g.compose(apow(g, elem, -1), apow(g, elem, n)) == apow(g, elem, n-1)
+    {
+        allApowClosed(g, elem);
+        if n > 0 {
+            calc {
+                g.compose(apow(g, elem, -1), apow(g, elem, n));
+                // == {apowPos(g,elem, n);}
+                g.compose(apow(g, elem, -1), g.compose(elem, apow(g, elem, n-1)));
+                g.compose(g.compose(apow(g, elem, -1), elem), apow(g, elem, n-1));
+                g.compose(g.compose(g.inverse(elem), elem), apow(g, elem, n-1));
+                g.compose(g.identity, apow(g, elem, n-1));
+                apow(g, elem, n-1);
+            }
+        }else if n == 0 {
+        }else{
+            assert n < 0;
+            assert (n-1)+1 == n;
+            calc {
+                g.compose(apow(g, elem, -1), apow(g, elem, n));
+                g.compose(apow(g, elem, -1), apow(g, elem, n));
+                g.compose(g.inverse(elem), apow(g, elem, n));
+                apow(g, elem, n-1);
+            }
+        }
+    }
 
+    lemma {:verify true} apowAddition<A>(g: Group<A>, elem: A, n: nat, k: nat)
+        requires elem in g.elements
+        requires ValidGroup(g)
+        ensures g.compose(apow(g, elem, n), apow(g, elem, k)) == apow(g, elem, n+k)
+    {
+        allApowClosed(g, elem);
+        if k == 0 {
+            assert apow(g, elem, k) == g.identity;
+            assert g.compose(apow(g, elem, n), g.identity) == apow(g, elem, n+k);
+        }else if n == 0 {
+            assert apow(g, elem, n) == g.identity;
+            assert g.compose(g.identity, apow(g, elem, k)) == apow(g, elem, n+k);
+        }else{
+            calc {
+                g.compose(apow(g, elem, n), apow(g, elem, k));
+                g.compose(g.compose(elem, apow(g, elem, n-1)), apow(g, elem, k));
+                g.compose(elem, g.compose(apow(g, elem, n-1), apow(g, elem, k)));
+                == {apowAddition(g,elem, n-1,k);}
+                g.compose(elem, apow(g, elem, n-1+k));
+                apow(g, elem, n+k);
+            }
+        }
+    }
+
+    lemma {:verify false} {:induction false} apowExponent<A>(g: Group<A>, elem: A, k: nat, s: nat)
+        requires elem in g.elements
+        requires ValidGroup(g)
+        ensures apow(g, apow(g, elem, k), s) == apow(g, elem, k*s);
+    {
+        allApowClosed(g,elem);
+        if s == 0 {
+            // assert apow(g,apow(g,elem,k),s) == g.identity;
+            assert k * s == 0;
+            assert s == 0;
+        }else{
+            calc {
+                apow(g, apow(g, elem, k), s);
+                g.compose(apow(g, elem, k), apow(g, apow(g, elem, k), s-1));
+                == {apowExponent(g, elem, k, s-1);}
+                g.compose(apow(g, elem, k), apow(g,elem, k*(s-1)));
+                == {apowAddition(g,elem, k, k*(s-1));}
+                apow(g, elem, k+k*(s-1));
+                apow(g, elem, k+k*s-k);
+                apow(g, elem, k*s);
+            }
+        }
+    }
+
+    predicate CyclicGroupGeneratedBy<A(!new)>(g: Group, elem: A)
+        requires elem in g.elements
+    {
+        exists n :: n == |g.elements| &&
+            apow(g, elem, n) == g.identity &&
+            (forall ns :: ns != n && apow(g, elem, ns) == g.identity ==> n < ns) &&
+            n != 0 &&
+            forall x :: x in g.elements && exists n :: apow(g, elem, n) == x
+    }
+
+    lemma {:verify false} AllSubgroupsOfCyclicSubgroupsAreCyclic<A(!new)>(g: Group, elem: A, h:Group)
+        requires elem in g.elements
+        requires CyclicGroupGeneratedBy(g, elem)
+        requires ValidGroup(g)
+        requires h.elements <= g.elements
+        requires ValidGroup(h)
+        requires ValidSubGroup(g, h)
+        ensures exists hx: A :: hx in h.elements && CyclicGroupGeneratedBy(h, hx)
+    {
+
+    }
+
+    export reveals *
 }
